\section*{Номер 107}
$$ 2u_xx + 5u_{yy} + 2u_{zz} -6u_{xy} -4 u_{xz} +6 u_{yz} - 3u + y - 2z = 0 $$
$$ 2x^2 + 5y^2 + 2z^2 - 6xy - 4xz + 6yz = 0 $$
$$ \begin{cases}
        x = t_1 + t_3 \\
        y = t_2       \\
        z = t_1 - t_3 \\
    \end{cases} \Rightarrow S_1 = \begin{vmatrix}
        1 & 0 & 1  \\
        0 & 1 & 0  \\
        1 & 0 & -1 \\
    \end{vmatrix}$$

$$ 2t_1^2 + 4t_1t_3 + t_3^2 + 5t_2^2 + 2t_1^2 - 4t_1t_3 + t_3^2 - 6t_1t_2 - 6t_2t_3 - 4t_1^2 + 4t_3^2 + 6t_1t_2 - 6t_2t_3 = $$
$$ = 8t_3^2 + 5t_2^2 - 12t_2t3 = 8\left(t_3 - \dfrac{3}{4}t_2\right)^2 + \dfrac{1}{2}t_2^2 = 0 $$
$$ \begin{cases}
        \eta = t_1                   \\
        \xi = -\dfrac{3}{4}t_2 + t_3 \\
        \mu = t_2                    \\
    \end{cases} \Rightarrow \begin{cases}
        t_1 = \eta                   \\
        t_2 = \mu                    \\
        t_3 = \dfrac{3}{4} \mu + \xi \\
    \end{cases} \Rightarrow S_2 = \begin{pmatrix}
        1 & 0 & 0           \\
        0 & 0 & 1           \\
        0 & 1 & \frac{3}{4} \\
    \end{pmatrix} $$

Теперь: $ \xi^2 + \dfrac{1}{2} \mu^2 = 0 $
$$ S_1 S_2 = \begin{pmatrix}
        1 & 1  & \dfrac{3}{4}  \\
        0 & 0  & 1             \\
        1 & -1 & -\dfrac{3}{4} \\
    \end{pmatrix} \Rightarrow \begin{cases}
        x = \eta + \xi + \dfrac{3}{4} \mu \\
        y = \mu                           \\
        z = \eta - \xi - \dfrac{3}{4} \mu \\
    \end{cases}$$

Производные:
$$ \begin{cases}
        u_x = \dfrac{1}{2} u_\eta + \dfrac{1}{2} u_\xi                                                                                                  \\
        u_y = -\dfrac{3}{4} u_\xi + u_\mu                                                                                                               \\
        u_z = \dfrac{1}{2} u_\eta - \dfrac{1}{2} u_\xi                                                                                                  \\
        u_{xx} = \dfrac{1}{4} u_{\eta \eta} + \dfrac{1}{4} u_{\xi \xi} + \dfrac{1}{2} u_{\eta \xi}                                                      \\
        u_{xy} = \dfrac{1}{2}\left(-\dfrac{3}{4} u_{\eta \xi} + u_{\eta \mu}\right) + \dfrac{1}{2} \left(-\dfrac{3}{4} u_{\xi \xi} + u_{\xi \mu}\right) \\
        u_{xz} = \dfrac{1}{4} (u_{\eta \eta} - u_{\xi \xi})                                                                                             \\
        u_{yz} = -\dfrac{3}{8} (u_{\xi \eta} - u_{\xi \xi}) + \dfrac{1}{2} (u_{\mu \eta} - u_{\mu \xi})                                                 \\
    \end{cases} $$

Подставим в исходное уравнение:
$$ 8u_{\xi \xi} + \dfrac{1}{2} u_{\mu \mu} - 3u + 2 \xi - 2 \eta + \dfrac{5}{2} \mu = 0 $$

\section*{Номер 102}
$$ u_{xx} - 4u_{xy} + 2u_{xz} + u_{zz} + 3u_x = 0 $$
$$ x^2 - 4xy + 2xz + z^2 = (x + z)^2 - 4xy = 0 $$
$$ \begin{cases}
    t_1 = x  \\
    t_2 = y \\
    t_3 = x + y \\
\end{cases} \Rightarrow t_3^2 - 4t_1 t_2 = 0$$

Получаем:
$$ \begin{cases}
    t_1 = \xi + \eta \\
    t_2 = \xi - \eta \\
    t_3 = \zeta \\
\end{cases} \Rightarrow \zeta^2 - 4\xi^2 + 4 \eta^2 = 0$$















% \section*{Номер 108}
% $$ 3u_{yy} - 2_{xy} - 2u_{yz} + 4u = 0 $$
% $$ 3y^2 - 2xy - 2yz = 0 \Rightarrow \begin{cases}
%     x = t_1 + t_2 \\
%     y = t_1 - t_2 \\
%     z = t_3  \\
% \end{cases}$$
% Имеем:
% $$ 3t_1^2 - 6t_1t_2 + 3t_2^2 - 2t_1^2 + t_2^2 - 2t_1t_3 + 2t_2t_3 = 0 $$











\section*{Номер 75}
$$ (1 + x^2)^2 u_{xx} + u_{yy} + 2x(1 + x^2)u_x = 0 $$
Характеристическое уравнение: $$ (1 + x^2)^2 \left(\dfrac{dy}{dx}\right)^2 + 1
    = 0 $$ $$ D = -4(1 + x^2)^2 < 0 $$ $$ dy = \pm \dfrac{i \sqrt{4(1 +
            x^2)^2}}{2(1 + x^2)}dx = \pm \dfrac{i}{1 + x^2}dx $$ $$ y = \pm i \arctan{x} +
    C $$ Сделаем замену: $$ \begin{cases}
        \xi = y \\
        \eta = \arctan{x}
    \end{cases} $$
Тогда:
$$ \begin{cases}
        u_{x} = u_\eta \eta_x' = u_\eta \dfrac{1}{1 + x^2}                                                                                                                                                          \\
        u_{y} = u_\xi \xi_y' = u_\xi                                                                                                                                                                                \\
        u_{xx} = \left(u_\eta \dfrac{1}{1 + x^2}\right)_x = u_{\eta \eta} \dfrac{1}{(1 + x^2)^2} + u_\eta \left(\dfrac{1}{1 + x^2}\right)_x = u_{\eta \eta} \dfrac{1}{(1 + x^2)^2} + u_\eta \dfrac{2x}{(1 + x^2)^2} \\
        u_{yy} = u_{\xi \xi}
    \end{cases} $$
Перепишем исходное уравнение:
$$ u_{\eta \eta} - 2x u_\eta + u_{\xi \xi} + 2x u_\eta = u_{\eta \eta} + u_{\xi \xi} $$

\section*{Номер 76}
$$ y^2 u_{xx} + 2xy u_{xy} + x^2 u_{yy} = 0 $$
Составим характеристическое уравнение:
$$ y^2 \left(\dfrac{dy}{dx}\right)^2 + 2xy \left(\dfrac{dy}{dx}\right) + x^2 = 0 $$
$$ D = 4x^2y^2 - 4 y^2 x^2 = 0 $$
$$ \dfrac{dy}{dx} = \dfrac{-2xy +\sqrt{0}}{2y^2} = -\dfrac{x}{y} $$
$$ y^2 = C + x^2 \Rightarrow y^2 - x^2 = C $$
Тогда:
$$ \begin{cases}
        \xi = y^2 - x^2 \\
        \eta = x        \\
    \end{cases} $$
$$ \begin{cases}
        u_x = u_\eta \eta_x = u_\eta \\
        u_y = u_\xi \xi_y = 2y u_\xi \\
        u_{xx} = -2u_\xi + 4
    \end{cases} $$

